pcuic/theories/PCUICCumulativity.v
@@ -309,22 +309,24 @@ Proof.
     eapply red_conv_conv_inv; eauto. now constructor.
 Qed.
 
-Definition conv_cum {cf:checker_flags} leq Σ Γ u v :=
-  match leq with
-  | Conv => ∥ Σ ;;; Γ |- u = v ∥
-  | Cumul => ∥ Σ ;;; Γ |- u <= v ∥
-  end.
-
-Definition conv_pb_rel {cf:checker_flags} (pb : conv_pb) :=
+Definition conv_pb_rel {cf:checker_flags} (pb : conv_pb) Σ :=
   match pb with
-  | Conv => eq_universe
-  | Cumul => leq_universe
+  | Conv => eq_universe Σ
+  | Cumul => leq_universe Σ
   end.
 
-Definition eq_termp_napp {cf:checker_flags} leq (Σ : global_env_ext) napp :=
-  eq_term_upto_univ_napp Σ (eq_universe Σ) (conv_pb_rel leq Σ) napp.
+Definition conv_pb_dir (pb : conv_pb) :=
+  match pb with
+  | Conv => false
+  | Cumul => true
+  end.
 
-Definition eq_termp {cf:checker_flags} leq Σ := (eq_termp_napp leq Σ 0).
+Coercion conv_pb_dir : conv_pb >-> bool.
+
+Definition eq_termp_napp {cf:checker_flags} (leq : conv_pb) (Σ : global_env_ext) napp :=
+  compare_term_napp leq Σ Σ napp.
+
+Notation eq_termp leq Σ := (compare_term (conv_pb_dir leq) Σ Σ).
 
 Lemma eq_term_eq_termp {cf:checker_flags} leq (Σ : global_env_ext) x y :
   eq_term Σ Σ x y ->
@@ -334,36 +336,6 @@ Proof.
   cbn.
   apply eq_term_upto_univ_leq; auto.
   typeclasses eauto.
-Qed.
-
-Lemma conv_cum_alt {cf:checker_flags} leq Σ Γ t t' :
-  conv_cum leq Σ Γ t t' <->
-  ∥∑ v v', (red Σ Γ t v × red Σ Γ t' v') × eq_termp leq Σ v v'∥.
-Proof.
-  assert (forall P Q, (P <~> Q) -> (∥P∥ <-> ∥Q∥)) by
-      (intros P Q H; split; intros [p]; constructor; apply H in p; auto).
-  destruct leq; cbn; apply H; [apply conv_alt_red|apply cumul_alt].
-Qed.
-
-Lemma conv_conv_cum_l {cf:checker_flags} :
-  forall (Σ : global_env_ext) leq Γ u v,
-      Σ ;;; Γ |- u = v ->
-      conv_cum leq Σ Γ u v.
-Proof.
-  intros Σ [] Γ u v h.
-  - cbn. constructor. assumption.
-  - cbn. constructor. now apply conv_cumul.
-Qed.
-
-Lemma conv_conv_cum_r {cf:checker_flags} :
-  forall (Σ : global_env_ext) leq Γ u v,
-      Σ ;;; Γ |- u = v ->
-      conv_cum leq Σ Γ v u.
-Proof.
-  intros Σ [] Γ u v h.
-  - cbn. constructor. apply conv_sym; auto.
-  - cbn. constructor. apply conv_cumul.
-    now apply conv_sym.
 Qed.
 
 Lemma cumul_App_l {cf:checker_flags} :
